Towards proving constructors and function calls.

LambdaS5/coq/LjsRulesCorrectDefinitions.v
@@ -778,13 +778,15 @@ Definition concl_expr_getvalue BR jst jc c st st' r je :=
 
 (** *** Theorem statements *)
 
-Definition th_expr k je := forall BR jst jc c st st' r, 
+Definition th_expr k je := 
+    forall BR jst jc c st st' r, 
     context_invariant BR jc c ->
     state_invariant BR jst st ->
     L.red_exprh k c st (L.expr_basic (js_expr_to_ljs je)) (L.out_ter st' r) ->
     concl_expr_getvalue BR jst jc c st st' r je.
 
-Definition th_stat k jt := forall BR jst jc c st st' r, 
+Definition th_stat k jt := 
+    forall BR jst jc c st st' r, 
     context_invariant BR jc c ->
     state_invariant BR jst st ->
     L.red_exprh k c st (L.expr_basic (js_stat_to_ljs jt)) (L.out_ter st' r) ->
@@ -815,6 +817,26 @@ Definition th_ext_expr_binary k v jeef P :=
     L.red_exprh k c st (L.expr_app_2 v [v1; v2]) (L.out_ter st' r) ->
     concl_ext_expr_value BR jst jc c st st' r (jeef jv1 jv2) P.
 
+Definition js_prealloc_callable jpre :=
+    match jpre with
+    | J.prealloc_global
+    | J.prealloc_math => False
+    | _ => True
+    end.
+
+Definition th_call_prealloc k jpre :=
+    forall BR jst jc c st st' r jv v jvs vs ptr ptr1 obj1,
+    js_prealloc_callable jpre ->
+    context_invariant BR jc c ->
+    state_invariant BR jst st ->
+    value_related BR jv v ->
+    values_related BR jvs vs ->
+    binds st ptr1 obj1 ->
+    arg_list_object obj1 vs ->
+    fact_js_obj (J.object_loc_prealloc jpre) ptr \in BR ->
+    L.red_exprh k c st (L.expr_app_2 (L.value_object ptr) [v; L.value_object ptr1]) (L.out_ter st' r) ->
+    concl_ext_expr_value BR jst jc c st st' r (J.spec_call_prealloc jpre jv jvs) (fun _ => True).
+
 (** *** Inductive hypotheses 
     The form of the induction hypotheses, as used in the proof. 
     Height induction is used to make proofs simpler. *)
@@ -822,3 +844,5 @@ Definition th_ext_expr_binary k v jeef P :=
 Definition ih_expr k := forall je k', (k' < k)%nat -> th_expr k' je.
 
 Definition ih_stat k := forall jt k', (k' < k)%nat -> th_stat k' jt.
+
+Definition ih_call_prealloc k := forall jpre k', (k' < k)%nat -> th_call_prealloc k' jpre.
