LambdaS5/coq/LjsRulesCorrectCallPrealloc.v
@@ -1,0 +1,56 @@
+Generalizable All Variables.
+Set Implicit Arguments.
+Require Import JsNumber.
+Require Import LjsShared.
+Require Import Utils.
+Require Import LjsRulesCorrectDefinitions.
+Require Import LjsRulesCorrectCommon.
+Require Import LjsRulesCorrectSpecFuns.
+Import ListNotations.
+Open Scope list_scope.
+Open Scope string_scope.
+
+Implicit Type A B : Type.
+Implicit Type s : string.
+Implicit Type n : number.
+Implicit Type i : L.id.
+Implicit Type st : L.store.
+Implicit Type e : L.expr.
+Implicit Type v : L.value.
+Implicit Type o : L.out.
+Implicit Type c : L.ctx.
+Implicit Type ptr : L.object_ptr.
+Implicit Type obj : L.object.
+Implicit Type re : L.result.
+Implicit Type r : L.res.
+Implicit Type props : L.object_props.
+
+Implicit Type jst : J.state.
+Implicit Type je : J.expr.
+Implicit Type jt : J.stat.
+Implicit Type jee : J.ext_expr.
+Implicit Type jet : J.ext_stat.
+Implicit Type jes : J.ext_spec.
+Implicit Type jc : J.execution_ctx.
+Implicit Type jo : J.out.
+Implicit Type jr : J.res.
+Implicit Type jv : J.value.
+Implicit Type jptr : J.object_loc.
+Implicit Type jobj : J.object.
+Implicit Type jrv : J.resvalue.
+Implicit Type jref : J.ref.
+Implicit Type jl : J.label.
+Implicit Type jer : J.env_record.
+Implicit Type jeptr : J.env_loc.
+Implicit Type jder : J.decl_env_record.
+Implicit Type jprops : J.object_properties_type.
+Implicit Type jlenv : J.lexical_env.
+
+Lemma red_expr_call_global_is_finite_ok : forall k, th_call_prealloc k J.prealloc_global_is_finite.
+Proof.
+Admitted.
+
+Lemma red_expr_call_global_is_nan_ok : forall k, th_call_prealloc k J.prealloc_global_is_nan.
+Proof.
+Admitted.
+
